Definition of the main datatypes and the sematics of the target language. Minor fixes on the definition of interfaces in the source language.

coq/simple-instance/target-language/Target.v
@@ -4,27 +4,180 @@ Require Export Source.
                   SYNTAX  
    _____________________________________ *)
 
-Definition memory : Type := list nat.
+Definition address : Type := nat.
 
-Definition register : Type := nat.
+(* For each component we have several procedures corresponding
+to an entry point address *)
+Definition entry_point : Type := address.
+Definition entry_points : Type := list (list entry_point).
 
-Definition registers : Type := list register.
+Definition fetch_entry_points 
+  (C:component_id) (P:procedure_id) (E:entry_points)
+  : entry_point :=
+  nth P (nth C E []) 0.
 
 Inductive binop : Type :=
-  | EAdd
-  | EMinus
-  | EMul.
+  | Add
+  | Minus
+  | Mul.
 
 Inductive instr : Type :=
   | Nop : instr
-  | Const : nat -> register -> instr
-  | Mov : register -> register -> instr
-  | BinOp : binop -> register -> register -> register -> instr
-  | Load : register -> register -> instr
-  | Store : register -> register -> instr
-  | Jal : register -> instr
-  | Jump : register -> instr
-  | Call : component -> procedure -> instr
+  | Const : nat -> address -> instr
+  | Mov : address -> address -> instr
+  | BinOp : binop -> address -> address -> address -> instr
+  | Load : address -> address -> instr
+  | Store : address -> address -> instr
+  | Jal : address -> instr
+  | Jump : address -> instr
+  | Call : component_id -> procedure_id -> instr
   | Return : instr
-  | Bnz : register -> nat -> instr
+  | Bnz : address -> nat -> instr
   | Halt : instr.
+
+Definition eval_binop (e : binop * nat * nat) : nat :=
+  match e with
+  | (Add, a, b) => a+b
+  | (Minus, a, b) => a-b
+  | (Mul, a, b) => a*b
+  end.
+
+Definition register : Type := nat.
+Definition registers : Type := list register. 
+
+(* Each component has it's own memory *)
+Definition memory : Type := list nat. 
+Definition global_memory : Type := list memory.
+
+Definition fetch_mem (C:component_id) (mem:global_memory) 
+  (a:address) : nat := 
+  nth C (nth a (mem) []) 0.
+
+Definition decode (n:nat) : option instr := admit.
+
+Definition encode (i:instr) : nat := admit.
+
+Theorem decode_encode :
+  forall (i:instr), decode (encode i) = Some i.
+Admitted.
+
+Definition procedure : Type :=
+  list instr.
+
+(* _____________________________________ 
+                SEMANTICS
+   _____________________________________ *)
+
+Inductive protected_call : Type := 
+  | PCall : component_id -> address -> protected_call.
+
+Definition protected_callstack : Type := 
+  list protected_call.
+
+Definition state : Type := 
+  (component_id * 
+   protected_callstack * 
+   global_memory * 
+   registers * 
+   address).
+
+Definition fetch_reg (a:address) (reg:registers) : register :=
+  nth a reg 0.
+
+Definition update_reg (a:address) (i:nat)
+  (reg:registers) : registers :=
+  update_value a i reg.
+
+Fixpoint update_mem (C:component_id) (mem:global_memory)
+  (a:address) (new:nat) : global_memory :=
+  match mem with
+  | [] => []
+  | h::t => match a with
+            | 0 => (update_value a new h) :: t
+            | S a' => h::(update_mem C mem a' new)
+            end
+  end.
+
+Reserved Notation "I ;; E |- s '⇒' s'" (at level 40).
+Inductive step (I:program_interfaces) (E:entry_points) : 
+  state -> state -> Prop :=
+  (* S_Nop *)
+  | S_Nop : forall mem C pc i d reg, 
+    (fetch_mem C mem pc = i) -> 
+    (decode i = Some Nop) -> 
+    I;;E |- (C,d,mem,reg,pc) ⇒ (C,d,mem,reg,pc+1)
+  (* S_Const *)
+  | S_Const : forall mem C pc i r i' d reg reg',
+    (fetch_mem C mem pc = i) ->
+    (decode i = Some (Const i' r)) ->
+    (update_reg r i' reg = reg') ->
+    I;;E |- (C,d,mem,reg,pc) ⇒ (C,d,mem,reg',pc+1)
+  (* S_Mov *)
+  | S_Mov : forall mem C pc i r1 r2 reg reg' d,
+    (fetch_mem C mem pc = i) ->
+    (decode i = Some (Mov r1 r2)) ->
+    (update_reg r2 (fetch_reg r1 reg) reg = reg') ->
+    I;;E |- (C,d,mem,reg,pc) ⇒ (C,d,mem,reg',pc+1)
+  (* S_BinOp *)
+  | S_BinOp : forall mem C pc i r1 r2 r3 reg reg' d op,
+    (fetch_mem C mem pc = i) ->
+    (decode i = Some (BinOp op r1 r2 r3)) ->
+    (update_reg r3 (eval_binop (op, (fetch_reg r1 reg), (fetch_reg r2 reg))) reg = reg') ->
+    I;;E |- (C,d,mem,reg,pc) ⇒ (C,d,mem,reg',pc+1)
+  (* S_Load *)
+  | S_Load : forall mem C pc i r1 r2 reg reg' d i1,
+    (fetch_mem C mem pc = i) ->
+    (decode i = Some (Load r1 r2)) ->
+    (fetch_reg r1 reg = i1) ->
+    (update_reg r2 (fetch_mem C mem i1) reg = reg') ->
+    I;;E |- (C,d,mem,reg,pc) ⇒ (C,d,mem,reg',pc+1)
+  (* S_Store *)
+  | S_Store : forall mem C pc i r1 r2 reg d i1 i2 mem',
+    (fetch_mem C mem pc = i) ->
+    (decode i = Some (Store r1 r2)) ->
+    (fetch_reg r1 reg = i1) ->
+    (fetch_reg r2 reg = i2) ->
+    (update_mem C mem i1 i2 = mem') ->
+    I;;E |- (C,d,mem,reg,pc) ⇒ (C,d,mem',reg,pc+1)
+  (* S_Jal *)
+  | S_Jal : forall mem C pc i i' r reg reg' d rra,
+    (fetch_mem C mem pc = i) ->
+    (decode i = Some (Jal r)) ->
+    (fetch_reg r reg = i') ->
+    (update_reg rra (pc+1) reg = reg') ->
+    I;;E |- (C,d,mem,reg,pc) ⇒ (C,d,mem,reg',i')
+  (* S_Call *)
+  | S_Call : forall mem C pc i reg d d' C' P',
+    (fetch_mem C mem pc = i) ->
+    (decode i = Some (Call C' P')) ->
+    (In (C',P') (get_import (nth C I (0,0,[]))) \/ C' = C) ->
+    (d' = (PCall C (pc+1))::d) ->
+    I;;E |- (C,d,mem,reg,pc) ⇒ (C',d',mem,reg,fetch_entry_points C' P' E)
+  (* S_Jump *)
+  | S_Jump : forall mem C pc i i' r reg d,
+    (fetch_mem C mem pc = i) ->
+    (decode i = Some (Jump r)) ->
+    (fetch_reg r reg = i') ->
+    I;;E |- (C,d,mem,reg,pc) ⇒ (C,d,mem,reg,i')
+  (* S_Return *)
+  | S_Return : forall mem C pc i i' d' reg d C',
+    (fetch_mem C mem pc = i) ->
+    (decode i = Some Return) ->
+    (d' = (PCall C' i')::d) ->
+    I;;E |- (C,d,mem,reg,pc) ⇒ (C',d',mem,reg,i')
+  (* S_BnzNZ *)
+  | S_BnzNZ : forall mem C pc i i' r reg d,
+    (fetch_mem C mem pc = i) ->
+    (decode i = Some (Bnz r i')) ->
+    ~(fetch_reg r reg = 0) ->
+    I;;E |- (C,d,mem,reg,pc) ⇒ (C,d,mem,reg,pc+1)
+  (* S_BnzZ *)
+  | S_BnzZ : forall mem C pc i i' r reg d,
+    (fetch_mem C mem pc = i) ->
+    (decode i = Some (Bnz r i')) ->
+    (fetch_reg r reg = 0) ->
+    I;;E |- (C,d,mem,reg,pc) ⇒ (C,d,mem,reg,pc+1)
+  where "I ;; E |- s '⇒' s'" := (step I E s s').
+
+  
+
